cv_translator/README.md
@@ -1,7 +1,13 @@
 Translator to cv type used by cv_compute
 
+[backend_32_cvScript.sml](backend_32_cvScript.sml):
+Translate arch-size-specific functions to cv equations.
+
 [backend_64_cvScript.sml](backend_64_cvScript.sml):
 Translate arch-size-specific functions to cv equations.
+
+[backend_ag32_cvScript.sml](backend_ag32_cvScript.sml):
+Translate arm8-specialised functions to cv equations.
 
 [backend_arm8_cvScript.sml](backend_arm8_cvScript.sml):
 Translate arm8-specialised functions to cv equations.
@@ -11,3 +17,6 @@ Translate non-target-specific backend functions to cv equations.
 
 [backend_x64_cvScript.sml](backend_x64_cvScript.sml):
 Translate x64-specialised functions to cv equations.
+
+[to_data_cvScript.sml](to_data_cvScript.sml):
+Translation of the to_data compiler function.
